Term/Lambda/LSimple.v
@@ -340,8 +340,6 @@ Module Type ST_Struct.
   Notation empty := (XMap.empty Ty).
   Notation Args := (@Args F X So typ).
 
-  (** Equivalence on environments. *)
-
   Infix "=&=" := (@Equal Ty) (at level 30).
 
 End ST_Struct.
@@ -358,225 +356,11 @@ Module Make (Export ST : ST_Struct).
 
 are finite maps from variables to types. *)
 
-  Require Import FMapFacts.
+  Require FMapUtil.
 
-  Module Export XMapFacts := Facts XMap.
-  Module Export XMapProps := Properties XMap.
-  Module Export XMapOrdProps := OrdProperties XMap.
-
-  Export XMap ST.
-
-  (** Inclusion ordering on environments. *)
-
-  Definition le (E F : En) := forall x T, MapsTo x T E -> MapsTo x T F.
-
-  Infix "<&=" := le (at level 40).
-
-  Instance le_refl : Reflexive le.
-
-  Proof. fo. Qed.
-
-  Instance le_trans : Transitive le.
-
-  Proof. intros E F G EF FG x T h. apply FG. apply EF. hyp. Qed.
-
-  Instance le_Equal : Proper (@Equal Ty ==> @Equal Ty ==> impl) le.
-
-  Proof.
-    intros E E' EE' F F' FF' EF x T hx.
-    rewrite <- FF'. apply EF. rewrite EE'. hyp.
-  Qed.
-
-  Lemma le_add : forall E x T, find x E = None -> E <&= add x T E.
-
-  Proof.
-    intros E x T hx y U hy. rewrite add_mapsto_iff. right. intuition.
-    subst y. rewrite find_mapsto_iff, hx in hy. discr.
-  Qed.
-
-  Instance MapsTo_le : Proper (Logic.eq ==> Logic.eq ==> le ==> impl)
-    (@MapsTo Ty).
-
-  Proof. intros x y xy T V TV E F EF h. subst y V. fo. Qed.
-
-  Instance In_le : Proper (Logic.eq ==> le ==> impl) (@In Ty).
-
-  Proof. intros x y xy E F EF [T h]. subst y. exists T. fo. Qed.
-
-  Instance add_le : Proper (XOrd.eq ==> Logic.eq ==> le ==> le) (@add Ty).
-
-  Proof.
-    intros x y xy T V TV E F EF. subst V. rewrite xy. intros z V.
-    do 2 rewrite find_mapsto_iff, add_o. eq_dec y z.
-    auto. do 2 rewrite <- find_mapsto_iff. rewrite EF. auto.
-  Qed.
-
-(****************************************************************************)
-(** ** Restriction of an environment to some set of variables. *)
-
-  Definition restrict_fun xs x (T:Ty) E :=
-    if XSet.mem x xs then add x T E else E.
-
-  Instance restrict_fun_e :
-    Proper (XSet.Equal ==> XOrd.eq ==> Logic.eq ==> Equal ==> Equal)
-      restrict_fun.
-
-  Proof.
-    intros xs xs' xsxs' x x' xx' T T' TT' E E' EE'. subst T'.
-    unfold restrict_fun. rewrite xx', xsxs'. destruct (XSet.mem x' xs').
-    rewrite xx', EE'. refl. hyp.
-  Qed.
-
-  Lemma restrict_fun_transp : forall xs,
-    transpose_neqkey Equal (restrict_fun xs).
-
-  Proof.
-    intros xs x x' T T' E h z. unfold restrict_fun.
-    destruct (XSet.mem x xs); destruct (XSet.mem x' xs); try refl.
-    rewrite !add_o. eq_dec x z; eq_dec x' z; try refl. subst. tauto.
-  Qed.
-
-  Definition restrict_dom E xs := fold (restrict_fun xs) E empty.
-
-  Lemma restrict_dom_empty : forall xs, Equal (restrict_dom empty xs) empty.
-
-  Proof.
-    intro xs. unfold restrict_dom. rewrite fold_Empty. refl. auto.
-    apply empty_1.
-  Qed.
-
-  Lemma restrict_dom_add : forall xs x T E, ~In x E ->
-    restrict_dom (add x T E) xs =&= restrict_fun xs x T (restrict_dom E xs).
-
-  Proof.
-    intros xs x T E hx. unfold restrict_dom. rewrite fold_add. refl. auto.
-    apply restrict_fun_e. refl. apply restrict_fun_transp. hyp.
-  Qed.
-
-  Instance restrict_dom_e : Proper (Equal ==> XSet.Equal ==> Equal)
-    restrict_dom.
-
-  Proof.
-    intro E; pattern E; apply map_induction_bis; clear E.
-    (* Equal *)
-    intros E E' EE' h F E'F xs xs' xsxs'. trans (restrict_dom E xs).
-    sym. apply h. hyp. refl. apply h. trans E'; hyp. hyp.
-    (* empty *)
-    intros E h xs xs' xsxs'. rewrite restrict_dom_empty. unfold restrict_dom.
-    rewrite fold_Empty. refl. auto. rewrite <- h. apply empty_1.
-    (* add *)
-    intros x T E hx h F e xs xs' xsxs'. rewrite restrict_dom_add. 2: hyp.
-    unfold restrict_dom at -1. rewrite <- (fold_Equal _ _ _ e).
-    rewrite fold_add; auto. apply restrict_fun_e; auto. apply h; auto. refl.
-    apply restrict_fun_e. refl. apply restrict_fun_transp.
-  Qed.
- 
-  Lemma mapsto_restrict_dom : forall E xs x T,
-    MapsTo x T (restrict_dom E xs) <-> (MapsTo x T E /\ XSet.In x xs).
-
-  Proof.
-    intro E; pattern E; apply map_induction_bis; clear E.
-    (* Equal *)
-    intros E E' EE' h xs x T. rewrite <- EE'. apply h.
-    (* empty *)
-    intros xs x T. rewrite restrict_dom_empty. rewrite empty_mapsto_iff. tauto.
-    (* add *)
-    intros x T E hx h xs y V. rewrite restrict_dom_add. 2: hyp.
-    unfold restrict_fun. case_eq (XSet.mem x xs).
-    do 2 rewrite add_mapsto_iff. rewrite h. rewrite mem_iff. intuition.
-    subst. hyp. 
-    rewrite add_mapsto_iff, h, <- not_mem_iff. intuition.
-    right. intuition. subst y. tauto.
-    subst. tauto.
-  Qed.
-
-  Instance restrict_dom_s : Proper (le ==> Subset ==> le) restrict_dom.
-
-  Proof.
-    intros E F EF xs xs' xsxs' x T. do 2 rewrite mapsto_restrict_dom.
-    rewrite <- xsxs', EF. auto.
-  Qed.
-
-  Lemma restrict_dom_le : forall E xs, restrict_dom E xs <&= E.
-
-  Proof. intros E xs y hy. rewrite mapsto_restrict_dom. tauto. Qed.
-
-  Lemma restrict_dom_singleton : forall E x,
-    restrict_dom E (singleton x) =&=
-    match find x E with None => empty | Some T => add x T empty end.
-
-  Proof.
-    intros E x. case_eq (find x E).
-    (* Some *)
-    intro T. rewrite <- find_mapsto_iff, Equal_mapsto_iff. intros hx y V.
-    rewrite mapsto_restrict_dom. set_iff.
-    rewrite add_mapsto_iff, empty_mapsto_iff.
-    intuition; subst. 2: hyp. left. intuition. eapply MapsTo_fun. apply hx. hyp.
-    (* None *)
-    rewrite <- not_find_in_iff, Equal_mapsto_iff. intros hx y V.
-    rewrite empty_mapsto_iff, mapsto_restrict_dom. set_iff. intuition.
-    apply hx. exists V. subst. hyp.
-  Qed.
-
-  Lemma mapsto_restrict_dom_singleton : forall x T E,
-    MapsTo x T E -> MapsTo x T (restrict_dom E (singleton x)).
-
-  Proof. intros x T E h. rewrite mapsto_restrict_dom. set_iff. auto. Qed.
-
-(****************************************************************************)
-(** ** Domain of a typing environment. *)
-
-  Definition dom_fun x (T:Ty) xs := XSet.add x xs.
-
-  Instance dom_fun_e :
-    Proper (Logic.eq ==> Logic.eq ==> XSet.Equal ==> XSet.Equal) dom_fun.
-
-  Proof.
-    intros x y xy T V TV s t st. subst. unfold dom_fun. rewrite st. refl.
-  Qed.
-
-  Lemma dom_fun_transp : transpose_neqkey XSet.Equal dom_fun.
-
-  Proof. intros x y xy T V E. unfold dom_fun. apply add_add. Qed.
-
-  Definition dom E := fold dom_fun E XSet.empty.
-
-  Instance dom_e : Proper (Equal ==> XSet.Equal) dom.
-
-  Proof.
-    intros E F EF. unfold dom. apply fold_Equal. fo. apply dom_fun_e. hyp.
-  Qed.
-
-  Lemma dom_empty : dom empty [=] XSet.empty.
-
-  Proof. unfold dom. rewrite fold_Empty. refl. fo. apply empty_1. Qed.
-
-  Lemma dom_add_notin : forall x T E,
-    ~In x E -> dom (add x T E) [=] XSet.add x (dom E).
-
-  Proof.
-    intros x T E h. unfold dom. rewrite fold_add. refl. fo. apply dom_fun_e.
-    apply dom_fun_transp. hyp.
-  Qed.
-
-  Lemma In_dom : forall x E, XSet.In x (dom E) <-> In x E.
-
-  Proof.
-    intros x E; pattern E; apply map_induction_bis; clear E.
-    (* Equal *)
-    intros E F EF h. rewrite <- EF. hyp.
-    (* empty *)
-    rewrite dom_empty, empty_in_iff. set_iff. refl.
-    (* add *)
-    intros y T E hy h. rewrite dom_add_notin. 2: hyp.
-    set_iff. rewrite add_in_iff, h. refl.
-  Qed.
-
-  Lemma dom_add : forall x T E, dom (add x T E) [=] XSet.add x (dom E).
-
-  Proof.
-    intros x T E y. rewrite In_dom, add_in_iff, <- In_dom. set_iff. refl.
-  Qed.
+  Module Export XMapUtil := FMapUtil.Make XMap.
+  Module Export Domain := XMapUtil.Domain XSet.
+  Import XMapUtil.
 
 (****************************************************************************)
 (** ** Typing. *)
@@ -625,9 +409,9 @@ are finite maps from variables to types. *)
     apply tr_app with V. apply IHtr1. tauto. apply IHtr2. tauto.
     apply tr_lam. eq_dec x y.
     (* x = y *)
-    subst y. eapply tr_le with (x:=add x X0 E).
-    intros z hz. do 2 rewrite find_mapsto_iff, add_o. rewrite remove_o.
-    eq_dec x z; auto. refl. refl. hyp.
+    eapply tr_le with (x:=add x X0 E). 2: refl. 2: refl.
+    intros z hz. do 2 rewrite find_mapsto_iff, add_o. eq_dec x z; auto.
+    rewrite remove_o. eq_dec y z. exfalso. apply n. trans y; hyp. auto. hyp.
     (* x <> y *)
     eapply tr_le with (x:= remove y (add x X0 E)). 2: refl. 2: refl.
     intros z hz. do 2 rewrite find_mapsto_iff. rewrite add_o.
@@ -738,12 +522,12 @@ are finite maps from variables to types. *)
 
     intros y V. unfold Def.single, Def.update.
     rewrite mapsto_restrict_dom, add_mapsto_iff. intros [h1 h2].
-    eq_dec y x.
-    subst y. assert (b : X0 = V). tauto. subst V.
+    eq_dec y x. unfold XSet.E.eq in e. subst.
+    assert (b : X0 = V). tauto. subst V.
     apply tr_var. rewrite add_mapsto_iff. auto.
     assert (b : MapsTo y V E). destruct h1. exfalso. apply n. sym. tauto. tauto.
     apply tr_var. rewrite add_mapsto_iff. eq_dec x1 y.
-    subst x1. tauto. tauto.
+    unfold XSet.E.eq in e. subst x1. tauto. tauto.
   Qed.
 
   Instance tr_aeq : Proper (Equal ==> aeq ==> Logic.eq ==> iff) tr.
